src/program_logic/staged_invariant_use_inuse.v
@@ -60,7 +60,7 @@ Proof.
   iEval (rewrite wpc0_unfold).
   rewrite /wpc_pre. iSplit; last first.
   {
-    iIntros (g1 ns D' κs) "Hg #HC".
+    iIntros (g1 ns D' κs) "Hg #HC Hlc".
     iDestruct (pri_inv_tok_disj with "[$]") as %[Hdisj|Hval]; last first.
     { exfalso. apply Qp.lt_nge in Hinvalid. revert Hval. rewrite frac_valid. eauto. }
     iMod (pri_inv_acc with "[$]") as "(Hinner&Hclo)".
@@ -114,7 +114,10 @@ Proof.
 
     rewrite /wpc_crash_modality.
     replace (⊤ ∖ D' ∖ E2) with (⊤ ∖ (E2 ∪ D')) by set_solver.
-    iSpecialize ("HPs" with "[$] [$]").
+    iDestruct (lc_weaken with "Hlc") as "Hlc".
+    { apply (num_laters_per_step_exp ns'). lia. }
+    iDestruct "Hlc" as "[[Hlc1 Hlc2] Hlc3]".
+    iSpecialize ("HPs" with "[$] [$] [$]").
     iMod "HPs".
     iModIntro. iApply (step_fupd2N_wand with "HPs"). iIntros "HPs".
     iMod "HPs" as "(Hg&HPr&HP)".
@@ -216,8 +219,8 @@ Proof.
         iModIntro. iIntros "Hwpc".
         assert (E1' = ⊤) as -> by set_solver.
         rewrite /wpc_crash_modality.
-        iIntros (????) "Hg HC".
-        iSpecialize ("Hwpc" with "[$] [$]").
+        iIntros (????) "Hg HC Hlc".
+        iSpecialize ("Hwpc" with "[$] [$] [$]").
         iApply (step_fupd2N_inner_wand with "Hwpc"); auto.
         iIntros "($&$)"; eauto.
       }
@@ -234,7 +237,7 @@ Proof.
         * iDestruct "Hv" as "(H&_)". iIntros.
           iDestruct (pri_inv_tok_global_le_acc _ _ _  mj_wp with "[] [$]") as "(Hg&Hg_clo)".
           { iPureIntro; naive_solver. }
-          iSpecialize ("H" with "[$] [$]").
+          iSpecialize ("H" with "[$] [$] [$]").
           iApply (step_fupd2N_inner_wand with "H"); auto.
           iIntros "(Hg&$)".
           iApply "Hg_clo". iFrame.
@@ -273,8 +276,8 @@ Proof.
       iModIntro. iIntros "Hwpc".
       iEval (rewrite wpc0_unfold) in "Hwpc". iDestruct "Hwpc" as "(_&Hwpc)".
       rewrite /wpc_crash_modality.
-      iIntros (????) "Hg HC".
-      iSpecialize ("Hwpc" with "[$] [$]").
+      iIntros (????) "Hg HC Hlc".
+      iSpecialize ("Hwpc" with "[$] [$] [$]").
       iApply (step_fupd2N_inner_wand with "Hwpc"); auto.
     }
     iDestruct ("Hg_inv_clo" with "Hg") as "Hg".
@@ -323,8 +326,8 @@ Proof.
   rewrite /wpc_pre. iSplit; last first.
   {
     iDestruct "Hwp" as "(Hwp&_)".
-    iIntros (g1 ns D' κs) "Hg #HC".
-    iSpecialize ("Hwp" $! mj with "[$] [$]").
+    iIntros (g1 ns D' κs) "Hg #HC Hlc".
+    iSpecialize ("Hwp" $! mj with "[$] [$] [$]").
     iApply (step_fupd2N_inner_wand with "Hwp"); auto.
   }
   rewrite Hnval.
@@ -435,8 +438,8 @@ Proof.
         iFrame.
         iModIntro. iIntros "Hwpc".
         rewrite /wpc_crash_modality.
-        iIntros (????) "Hg HC".
-        iSpecialize ("Hwpc" with "[$] [$]").
+        iIntros (????) "Hg HC Hlc".
+        iSpecialize ("Hwpc" with "[$] [$] [$]").
         iApply (step_fupd2N_inner_wand with "Hwpc"); auto.
         iIntros "($&$)"; eauto.
       }
@@ -455,7 +458,7 @@ Proof.
             etransitivity; first eapply Qp.le_min_l.
             etransitivity; first eapply Qp.le_min_l.
             eapply Qp.le_min_r. }
-          iSpecialize ("H" with "[$] [$]").
+          iSpecialize ("H" with "[$] [$] [$]").
           iApply (step_fupd2N_inner_wand with "H"); auto.
           iIntros "(Hg&$)".
           iApply "Hg_clo". iFrame.
@@ -511,8 +514,8 @@ Proof.
     iModIntro. iIntros "Hwpc".
     iEval (rewrite wpc0_unfold) in "Hwpc". iDestruct "Hwpc" as "(_&Hwpc)".
     rewrite /wpc_crash_modality.
-    iIntros (????) "Hg HC".
-    iSpecialize ("Hwpc" with "[$] [$]").
+    iIntros (????) "Hg HC Hlc".
+    iSpecialize ("Hwpc" with "[$] [$] [$]").
     iApply (step_fupd2N_inner_wand with "Hwpc"); auto.
   }
   iDestruct ("Hg_inv_clo" with "Hg") as "Hg".
